improvement: move some definitions

theories/rust_typing/ltypes.v
@@ -20,324 +20,6 @@ Proof. rewrite (UIP_refl _ _ Heq). done. Qed.
 
 (** * Place types *)
 
-Section place_rfn.
-  Context `{!typeGS Σ}.
-
-  (**
-    [PlaceIn]: the current inner refinement is accurate (no blocking of the inner refinement).
-[PlaceGhost]: the current inner refinement is determined by a ghost variable, either because it is currently blocked or was implicitly unblocked.
-  *)
-  Inductive place_rfn_mode := PlaceModeIn | PlaceModeGhost.
-  (* concrete refinements *)
-  Inductive place_rfn (rt : Type) :=
-    | PlaceIn (r : rt)
-    | PlaceGhost (γ : gname).
-  Global Arguments PlaceIn {_}.
-  Global Arguments PlaceGhost {_}.
-
-  Definition place_rfnRT (rt : RT) : RT :=
-    mk_RT (place_rfn (RT_rt rt))%type (RT_xt rt) (PlaceIn ∘ RT_xrt rt).
-  Canonical Structure place_rfnRT.
-
-  Global Instance place_rfn_inh rt : Inhabited (place_rfn rt).
-  Proof. refine (populate (PlaceGhost inhabitant )). Qed.
-  Global Instance place_rfn_mode_inh : Inhabited (place_rfn_mode).
-  Proof. refine (populate (PlaceModeGhost)). Qed.
-
-  (* interpretation of place_rfn under owned *)
-  Definition place_rfn_interp_owned {rt} (r : place_rfn rt) (r' : rt) : iProp Σ :=
-    match r with
-    | PlaceIn r'' => ⌜r'' = r'⌝
-    | PlaceGhost γ' => gvar_pobs γ' r'
-    end.
-
-  Definition place_rfn_interp_owned_blocked {rt} (r : place_rfn rt) (r' : rt) : iProp Σ :=
-    match r with
-    | PlaceIn r'' => ⌜r'' = r'⌝
-    | PlaceGhost γ' => gvar_auth γ' r'
-    end.
-
-  (* interpretation of place_rfn under mut *)
-  Definition place_rfn_interp_mut {rt} (r : place_rfn rt) γ : iProp Σ :=
-    match r with
-    | PlaceIn r' => gvar_obs γ r'
-    | PlaceGhost γ' => Rel2 γ' γ (@eq rt)
-    end.
-  Definition place_rfn_interp_mut_blocked {rt} (r : place_rfn rt) γ : iProp Σ :=
-    match r with
-    | PlaceIn r' => gvar_obs γ r'
-    | PlaceGhost γ' => Rel2 γ' γ (@eq rt)
-    end.
-
-  (* interpretation of place_rfn under shared *)
-  (* we don't get any knowledge for PlaceGhost: we should really unblock before initiating sharing *)
-  Definition place_rfn_interp_shared {rt} (r : place_rfn rt) (r' : rt) : iProp Σ :=
-    match r with
-    | PlaceIn r'' => ⌜r'' = r'⌝
-    | PlaceGhost γ => gvar_pobs γ r'
-    end.
-  Global Instance place_rfn_interp_shared_pers {rt} (r : place_rfn rt) r' : Persistent (place_rfn_interp_shared r r').
-  Proof. destruct r; apply _. Qed.
-  (* NOTE: It's a bit unlucky that we have to rely on timelessness of this in some cases, in particular for some of the unfolding lemmas. *)
-  (* Global Instance place_rfn_interp_shared_timeless {rt} (r : place_rfn rt) r' : Timeless (place_rfn_interp_shared r r'). *)
-  (* Proof. destruct r; apply _. Qed. *)
-  Global Instance place_rfn_interp_owned_timeless {rt} (r : place_rfn rt) r' : Timeless (place_rfn_interp_owned r r').
-  Proof. destruct r; apply _. Qed.
-  Global Instance place_rfn_interp_mut_timeless {rt} (r : place_rfn rt) γ : Timeless (place_rfn_interp_mut r γ).
-  Proof. destruct r; apply _. Qed.
-
-  Lemma place_rfn_interp_mut_iff {rt} (r : place_rfn rt) γ :
-    place_rfn_interp_mut r γ ⊣⊢ ∃ r' : rt, gvar_obs γ r' ∗ match r with | PlaceGhost γ' => gvar_pobs γ' r' | PlaceIn r => ⌜r = r'⌝ end.
-  Proof.
-    destruct r as [ r | γ']; simpl.
-    - iSplit.
-      + iIntros "?"; eauto with iFrame.
-      + iIntros "(%r' & ? & ->)"; iFrame.
-    - iSplit.
-      + iIntros "(%r1 & %r2 & ? & ? & ->)". iExists _. iFrame.
-      + iIntros "(%r' & ? & ?)". iExists _, _. iFrame. done.
-  Qed.
-
-  Lemma place_rfn_interp_mut_owned {rt} (r : place_rfn rt) (r' : rt) γ :
-    place_rfn_interp_mut r γ -∗
-    gvar_auth γ r' ==∗
-    place_rfn_interp_owned r r' ∗
-    gvar_obs γ r' ∗ gvar_auth γ r'.
-  Proof.
-    iIntros "Hrfn Hauth".
-    destruct r as [r'' | γ']; simpl.
-    - iPoseProof (gvar_agree with "Hauth Hrfn") as "#->".
-      iSplitR; first done. by iFrame.
-    - iDestruct "Hrfn" as "(%r1 & %r2 & Hauth' & Hobs & ->)".
-      iPoseProof (gvar_agree with "Hauth Hobs") as "#->". iFrame. done.
-  Qed.
-  Lemma place_rfn_interp_owned_mut {rt} (r : place_rfn rt) r' γ :
-    place_rfn_interp_owned r r' -∗
-    gvar_obs γ r' -∗
-    place_rfn_interp_mut r γ.
-  Proof.
-    iIntros "Hrfn Hobs".
-    destruct r as [r'' | γ'].
-    - iDestruct "Hrfn" as "<-". iFrame.
-    - iDestruct "Hrfn" as "Hauth'". simpl.
-      rewrite /Rel2. iExists _, _. by iFrame.
-  Qed.
-
-  (** lemmas for unblocking *)
-  Lemma place_rfn_interp_owned_blocked_unblock {rt} (r : place_rfn rt) (r' : rt) :
-    place_rfn_interp_owned_blocked r r' ==∗ place_rfn_interp_owned r r'.
-  Proof.
-    destruct r as [ r'' | γ]; simpl; first by eauto.
-    iApply gvar_auth_persist.
-  Qed.
-  Lemma place_rfn_interp_mut_blocked_unblock {rt} (r : place_rfn rt) (γ : gname) :
-    place_rfn_interp_mut_blocked r γ ==∗ place_rfn_interp_mut r γ.
-  Proof.
-    destruct r as [ r' | γ']; simpl; first by eauto.
-    eauto.
-  Qed.
-
-  (** lemmas for sharing *)
-  Lemma place_rfn_interp_owned_share' {rt} (r : place_rfn rt) (r' : rt) :
-    place_rfn_interp_owned r r' -∗
-    place_rfn_interp_shared r r'.
-  Proof.
-    iIntros "Hrfn".
-    destruct r.
-    - iDestruct "Hrfn" as "->". eauto.
-    - iDestruct "Hrfn" as "#Hrfn". eauto.
-  Qed.
-  Lemma place_rfn_interp_owned_share F {rt} (r : place_rfn rt) (r' : rt) q κ :
-    lftE ⊆ F →
-    lft_ctx -∗
-    &{κ} (place_rfn_interp_owned r r') -∗
-    q.[κ] ={F}=∗
-    place_rfn_interp_shared r r' ∗ q.[κ].
-  Proof.
-    iIntros (?) "#LFT Hb Htok".
-    iMod (bor_acc with "LFT Hb Htok") as "(>Hrfn & Hcl)"; first solve_ndisj.
-    iPoseProof (place_rfn_interp_owned_share' with "Hrfn") as "#Hrfn'".
-    iMod ("Hcl" with "[//]") as "(? & $)". eauto.
-  Qed.
-  Lemma place_rfn_interp_mut_share' (F : coPset) {rt : RT} `{!Inhabited rt} (r : place_rfn rt) (r' : rt) γ (q : Qp) κ :
-    lftE ⊆ F →
-    lft_ctx -∗
-    place_rfn_interp_mut r γ -∗
-    &{κ} (gvar_auth γ r') -∗
-    q.[κ] ={F}=∗
-    place_rfn_interp_shared r r' ∗ (▷ place_rfn_interp_mut r γ) ∗ &{κ} (gvar_auth γ r') ∗ q.[κ].
-  Proof.
-    iIntros (?) "#CTX Hobs Hauth Htok".
-    iMod (bor_acc with "CTX Hauth Htok") as "(>Hauth & Hcl_auth)"; first solve_ndisj.
-    iAssert (|={F}=> place_rfn_interp_shared r r' ∗ gvar_auth γ r' ∗ ▷ place_rfn_interp_mut r γ)%I with "[Hauth Hobs]" as ">(Hrfn & Hauth & Hobs)".
-    { destruct r.
-      - iDestruct "Hobs" as "Hobs". iPoseProof (gvar_agree with "Hauth Hobs") as "#->". eauto with iFrame.
-      - simpl. rewrite /Rel2. iDestruct "Hobs" as "(%v1 & %v2 & #Hpobs & Hobs & %Heq')". rewrite Heq'.
-        iPoseProof (gvar_agree with "Hauth Hobs") as "%Heq". rewrite Heq.
-        iFrame. iR. iModIntro. iModIntro. iExists _. iR. done.
-    }
-    iMod ("Hcl_auth" with "[$Hauth]") as "($ & Htoka2)".
-    by iFrame.
-  Qed.
-  Lemma place_rfn_interp_mut_share (F : coPset) {rt : RT} `{!Inhabited rt} (r : place_rfn rt) (r' : rt) γ (q : Qp) κ :
-    lftE ⊆ F →
-    lft_ctx -∗
-    &{κ} (place_rfn_interp_mut r γ) -∗
-    &{κ} (gvar_auth γ r') -∗
-    q.[κ] ={F}=∗
-    place_rfn_interp_shared r r' ∗ &{κ} (place_rfn_interp_mut r γ) ∗ &{κ} (gvar_auth γ r') ∗ q.[κ].
-  Proof.
-    iIntros (?) "#CTX Hobs Hauth (Htok1 & Htok2)".
-    iMod (bor_acc with "CTX Hobs Htok1") as "(>Hobs & Hcl_obs)"; first solve_ndisj.
-    iMod (place_rfn_interp_mut_share' with "CTX Hobs Hauth Htok2") as "($ & Hmut & $ & $)"; first done.
-    iMod ("Hcl_obs" with "[$Hmut]") as "($ & Htok_κ')".
-    by iFrame.
-  Qed.
-
-  Lemma place_rfn_interp_shared_mut {rt} (r : place_rfn rt) r' γ :
-    place_rfn_interp_shared r r' -∗
-    gvar_obs γ r' -∗
-    place_rfn_interp_mut r γ.
-  Proof.
-    iIntros "Hrfn Hobs".
-    destruct r as [ r | γ']; simpl.
-    - iDestruct "Hrfn" as "<-"; eauto with iFrame.
-    - iExists _, _. eauto with iFrame.
-  Qed.
-  Lemma place_rfn_interp_shared_owned {rt} (r : place_rfn rt) r' :
-    place_rfn_interp_shared r r' -∗
-    place_rfn_interp_owned r r'.
-  Proof. destruct r; eauto with iFrame. Qed.
-
-
-  (** For adding information to the context *)
-  Definition place_rfn_interp_mut_extracted {rt} (r : place_rfn rt) (γ : gname) : iProp Σ :=
-    match r with
-    | PlaceIn r' => gvar_pobs γ r'
-    | PlaceGhost γ' => Rel2 (T:=rt) γ' γ eq
-    end.
-  Definition place_rfn_interp_owned_extracted {rt} (r : place_rfn rt) (r' : rt) : iProp Σ :=
-    match r with
-    | PlaceIn r'' => ⌜r'' = r'⌝
-    | PlaceGhost γ' => gvar_pobs γ' r'
-    end.
-
-  Lemma place_rfn_interp_mut_extract {rt} (r : place_rfn rt) (γ : gname) :
-    place_rfn_interp_mut r γ ==∗ place_rfn_interp_mut_extracted r γ.
-  Proof.
-    destruct r; simpl.
-    - iIntros "Hobs". iApply (gvar_obs_persist with "Hobs").
-    - eauto.
-  Qed.
-  Lemma place_rfn_interp_owned_extract {rt} (r : place_rfn rt) (r' : rt) :
-    place_rfn_interp_owned r r' ==∗ place_rfn_interp_owned_extracted r r'.
-  Proof.
-    destruct r; simpl.
-    - eauto.
-    - eauto.
-  Qed.
-End place_rfn.
-
-(** ** Basic enum infrastructure *)
-Section enum.
-  Context `{!typeGS Σ}.
-
-  Record enum_tag_sem {rt : Type} := mk_enum_tag_sem {
-    enum_tag_sem_rt : RT;
-    enum_tag_sem_ty : type enum_tag_sem_rt;
-    enum_tag_rt_inj : enum_tag_sem_rt → rt;
-  }.
-  Global Arguments enum_tag_sem : clear implicits.
-  Global Arguments mk_enum_tag_sem {_}.
-
-  Record enum (rt : RT) : Type := _mk_enum {
-    enum_xt_inhabited : Inhabited (RT_xt rt);
-    (* the layout spec *)
-    enum_els : enum_layout_spec;
-    (* out of the current refinement, extract the tag *)
-    enum_tag : rt → option var_name;
-    (* out of the current refinement, extract the component type and refinement *)
-    enum_rt : rt → RT;
-    enum_ty : ∀ r, type (enum_rt r);
-    enum_r : ∀ r, enum_rt r;
-    (* convenience function: given the variant name, also project out the type *)
-    enum_tag_ty_inj :
-      var_name →
-      option (enum_tag_sem rt);
-    (* explicitly track the lifetimes each of the variants needs -- needed for sharing *)
-    enum_lfts : list lft;
-    enum_wf_E : elctx;
-    enum_lfts_complete : ∀ (r : rt), ty_lfts (enum_ty r) ⊆ enum_lfts;
-    enum_wf_E_complete : ∀ (r : rt), ty_wf_E (enum_ty r) ⊆ enum_wf_E;
-    enum_tag_compat : ∀ (r : rt) (variant : var_name),
-      enum_tag r = Some variant →
-      (*enum_tag_ty_inj variant = Some (mk_enum_tag_sem (enum_rt r) (enum_ty r));*)
-      sigT (λ vinj, enum_tag_ty_inj variant = Some (mk_enum_tag_sem (enum_rt r) (enum_ty r) vinj));
-  }.
-  Global Arguments _mk_enum {_}.
-  Global Arguments enum_xt_inhabited {_}.
-  Global Arguments enum_els {_}.
-  Global Arguments enum_tag {_}.
-  Global Arguments enum_rt {_}.
-  Global Arguments enum_r {_}.
-  Global Arguments enum_ty {_}.
-  Global Arguments enum_tag_ty_inj {_}.
-  Global Arguments enum_lfts {_}.
-  Global Arguments enum_wf_E {_}.
-  Global Instance enum_rt_inhabited {rt} (e : enum rt) : Inhabited rt :=
-    populate (RT_xrt rt e.(enum_xt_inhabited).(inhabitant)).
-
-  (* Block TC resolution from solving the [Inhabited] requirement automatically to make automation more deterministic *)
-  Definition mk_enum {rt : RT} (inh : TCNoResolve (Inhabited (RT_xt rt))) := _mk_enum inh.
-
-
-  Definition enum_tag' {rt} (en : enum rt) (r : rt) : string :=
-    default "" (enum_tag en r).
-
-  Definition enum_lookup_tag {rt} (e : enum rt) (r : rt) : option Z :=
-    fmap (els_lookup_tag e.(enum_els)) (e.(enum_tag) r).
-
-  Definition size_of_enum_data (els : enum_layout_spec) :=
-    ly_size (use_union_layout_alg' (uls_of_els els)).
-
-  Definition els_data_ly (els : enum_layout_spec) :=
-    use_union_layout_alg' (uls_of_els els).
-
-  Import EqNotations.
-  Lemma enum_tag_rt_eq {rt} (en : enum rt) r tag sem :
-    enum_tag en r = Some tag →
-    enum_tag_ty_inj en tag = Some sem →
-    sem.(enum_tag_sem_rt) = enum_rt en r.
-  Proof.
-    intros Htag Hsem.
-    odestruct (enum_tag_compat _ en) as (vinj & Htg); first done.
-    simplify_eq. done.
-  Defined.
-
-  Lemma enum_tag_type_eq {rt} (en : enum rt) r tag sem
-    (Heq : enum_tag en r = Some tag)
-    (Hsem : enum_tag_ty_inj en tag = Some sem) :
-    sem.(enum_tag_sem_ty) =
-    rew <-[type] (enum_tag_rt_eq en r _ _ Heq Hsem) in enum_ty en r.
-  Proof.
-    odestruct (enum_tag_compat _ en) as (vinj & Htg); first done.
-    simplify_eq.
-    generalize (enum_tag_rt_eq en r tag _ Heq Hsem) as Heq2.
-    simpl. intros Heq2. rewrite (UIP_refl _ _ Heq2); done.
-  Qed.
-  Lemma enum_tag_type_eq' {rt} (en : enum rt) r tag sem
-    (Heq : enum_tag en r = Some tag)
-    (Hsem : enum_tag_ty_inj en tag = Some sem) :
-    rew ->[type] (enum_tag_rt_eq en r _ _ Heq Hsem) in sem.(enum_tag_sem_ty) =
-    enum_ty en r.
-  Proof.
-    odestruct (enum_tag_compat _ en) as (vinj & Htg); first done.
-    simplify_eq.
-    generalize (enum_tag_rt_eq en r tag _ Heq Hsem) as Heq2.
-    simpl. intros Heq2. rewrite (UIP_refl _ _ Heq2); done.
-  Qed.
-End enum.
-
 Section array.
   Context `{!typeGS Σ}.
   Section list_map.
@@ -1260,9 +942,6 @@ Section ltype_def.
   Definition lty_own_type_rec (lt0 : lty) := ∀ lt : lty, bor_kind → thread_id → place_rfn (lty_rt lt) → loc → lty_size_rel lt lt0 → iProp Σ.
 
   Definition UninitLty st := OfTyLty (uninit st).
-
-  Definition maybe_creds (wl : bool) := (if wl then £ num_cred ∗ atime 1 else True)%I.
-  Definition have_creds : iProp Σ := £ num_cred ∗ atime 1.
 
   Definition lty_of_ty_own {rt} (ty : type rt) k π (r : place_rfn rt) l :=
     (∃ ly : layout, ⌜syn_type_has_layout ty.(ty_syn_type) ly⌝ ∗ ⌜l `has_layout_loc` ly⌝ ∗
@@ -2567,7 +2246,7 @@ Section ltype_def.
       + unshelve iApply lty_own_to_core_ofty; [ | done | done | ]. done.
       + unshelve iPoseProof (IH with "Hl") as "Hl"; [ | | done | ].
         { by rewrite lty_core_rt_eq. }
-        iApply (lty_own_pre_rfn_eq with "Hl"). 
+        iApply (lty_own_pre_rfn_eq with "Hl").
         (*apply rew_swap. rewrite rew_compose rew_UIP_RT//.*)
         admit.
     - (* enum *)
@@ -4485,10 +4164,6 @@ Section ltype_def.
   Qed.
 End ltype_def.
 
-Notation "# x" := (PlaceIn x) (at level 9) : stdpp_scope.
-Notation "'<#>' x" := (fmap (M := list) PlaceIn x) (at level 30).
-Notation "'<#>@{' A '}' x" := (fmap (M := A) PlaceIn x) (at level 30).
-Notation "👻 γ" := (PlaceGhost γ) (at level 9) : stdpp_scope.
 Notation "◁ ty" := (OfTy ty) (at level 15) : bi_scope.
 
 Notation "l ◁ₗ[ π , k ]  r  @  ty" := (ltype_own ty k π r l) (at level 15) : bi_scope.
@@ -5488,11 +5163,11 @@ Section blocked.
           apply pad_struct_lookup_Some in Hlook; first last.
           { rewrite length_hpzipl -Hlen. erewrite struct_layout_spec_has_layout_fields_length;done. }
           destruct Hlook as (n & ly' & Hlook & [(? & Hlook1) | (-> & Hlook1)]).
-          { simpl in *. 
+          { simpl in *.
             apply (hpzipl_lookup_inv_hzipl_pzipl _ _ r') in Hlook1 as (Hlook1 & _).
             iPoseProof (big_sepL_lookup with "Hub") as "Hub'"; first done. simpl.
             iDestruct "Hub'" as "(_ & #Hub_own)". iMod ("Hub_own" with "Hdead Hl") as "Hl".
-            rewrite ltype_own_core_equiv. rewrite ltype_core_syn_type_eq. eauto 8 with iFrame. 
+            rewrite ltype_own_core_equiv. rewrite ltype_core_syn_type_eq. eauto 8 with iFrame.
           }
           { (* uninit *)
             injection Hlook1 => _ _ ?. subst.
@@ -5548,7 +5223,7 @@ Section blocked.
       apply pad_struct_lookup_Some in Hlook; first last.
       { rewrite length_hpzipl -Hlen. erewrite struct_layout_spec_has_layout_fields_length;done. }
       destruct Hlook as (n & ly' & Hlook & [(? & Hlook1) | (-> & Hlook1)]).
-      { 
+      {
         apply (hpzipl_lookup_inv_hzipl_pzipl _ _ r') in Hlook1 as (Hlook1 & _).
         iPoseProof (big_sepL_lookup with "Hub") as "Hub'"; first done. simpl.
         iDestruct "Hub'" as "(_ & #Hub_own)". iMod ("Hub_own" with "Hdead Hl") as "Hl".
