theories/rust_typing/shr_ref/unfold.v
@@ -4,6 +4,22 @@ From refinedrust.shr_ref Require Import def subltype.
 From refinedrust Require Import options.
 
 (** ** Unfolding [shr_ref] into [ShrLtype] *)
+Section ofty.
+  Context `{!typeGS Σ}.
+
+  (** A very fundamental equivalence that should hold *)
+  Lemma shr_ref_ofty_shared_equiv {rt} (ty : type rt) π κ l r :
+    l ◁ₗ[π, Shared κ] #r @ (◁ ty) ⊣⊢ l ◁ᵥ{π} #r @ shr_ref κ ty.
+  Proof.
+    rewrite ltype_own_ofty_unfold/lty_of_ty_own /ty_own_val/=.
+    iSplit.
+    - iIntros "(%ly & %Hst & %Hly & #Hsc & #Hlb & %r' & <- & #Ha)".
+      iExists _, _, _. iR. iR. iR. iFrame "#". done.
+    -iIntros "(%l' & %ly & %r' & %Hl & % & % & #Hsc & #Hlb & <- & #Ha)".
+      apply val_of_loc_inj in Hl. subst.
+      iExists _. iR. iR. iFrame "#". done.
+  Qed.
+End ofty.
 
 Section ltype_agree.
   Context `{typeGS Σ}
